Make safechecker compute (#682)
* make eqb compute

* change some Qed's to Defined

* test file

* Fix definition of equality of terms, contexts etc in PCUIC to be efficient and transparent

* add fuel to isconf_full and fix other computation issues

* correct ReflectEq for case_info

* remove useless and dangerous instance of EqDec_ReflectEq

* more uniform treatment of Reflect

* make recursive calls compute in SafeConversion

* clean up computational content

* make guard compute

* typecheck_program build the environement

* add more tests in test-suite

* fix plugin generation

* more computation

* add missing import

Co-authored-by: Matthieu Sozeau <mattam@mattam.org>
(cherry picked from commit 105e0ea9f4294d558f183e9fb978c7257cd40b43)

template-coq/theories/Reflect.v
@@ -1,7 +1,7 @@
 (* Distributed under the terms of the MIT license. *)
 (* For primitive integers and floats  *)
 From Coq Require Numbers.Cyclic.Int63.Uint63 Floats.PrimFloat Floats.FloatAxioms.
-From MetaCoq.Template Require Import utils BasicAst Universes.
+From MetaCoq.Template Require Import utils BasicAst Universes Kernames.
 Require Import ssreflect.
 From Equations Require Import Equations.
 
@@ -12,12 +12,12 @@ Next Obligation.
   now apply (Numbers.Cyclic.Int63.Uint63.eqb_spec x y) in eq.
   now apply (Numbers.Cyclic.Int63.Uint63.eqb_false_spec x y) in eq.
 Qed.
- 
+
 Derive NoConfusion EqDec for SpecFloat.spec_float.
 
 Local Obligation Tactic := idtac.
 
-#[program,global] 
+#[program,global]
 Instance reflect_prim_float : ReflectEq PrimFloat.float :=
   { eqb x y := eqb (ReflectEq := EqDec_ReflectEq SpecFloat.spec_float) (FloatOps.Prim2SF x) (FloatOps.Prim2SF y) }.
 Next Obligation.
@@ -43,7 +43,7 @@ Next Obligation.
   all: unfold eq_prop_level.
   all: try solve [ constructor ; reflexivity ].
   all: try solve [ constructor ; discriminate ].
-Defined.
+Qed.
 
 Definition eq_levels (l1 l2 : PropLevel.t + Level.t) :=
   match l1, l2 with
@@ -61,7 +61,7 @@ Next Obligation.
   all:try (constructor; cong).
   cbn -[eqb]. destruct (eqb_spec t t0). subst; now constructor.
   constructor; cong.
-Defined.
+Qed.
 
 
 Definition eq_name na nb :=
@@ -81,7 +81,7 @@ Next Obligation.
   - cbn. constructor. discriminate.
   - unfold eq_name. destruct (eqb_spec i i0); nodec.
     constructor. f_equal. assumption.
-Defined.
+Qed.
 
 Definition eq_relevance r r' :=
   match r, r' with
@@ -99,12 +99,12 @@ Next Obligation.
   - cbn. constructor. discriminate.
   - cbn. constructor. discriminate.
   - simpl. now constructor.
-Defined.
+Qed.
 
 Definition eq_aname (na nb : binder_annot name) :=
   eqb na.(binder_name) nb.(binder_name) &&
   eqb na.(binder_relevance) nb.(binder_relevance).
-  
+
 #[global, program] Instance reflect_aname : ReflectEq aname := {
   eqb := eq_aname
 }.
@@ -113,7 +113,7 @@ Next Obligation.
   destruct (eqb_spec x.(binder_name) y.(binder_name));
   destruct (eqb_spec x.(binder_relevance) y.(binder_relevance));
   constructor; destruct x, y; simpl in *; cong.
-Defined.
+Qed.
 
 Definition eq_def {A} `{ReflectEq A} (d1 d2 : def A) : bool :=
   match d1, d2 with
@@ -133,7 +133,7 @@ Next Obligation.
   destruct (eqb_spec b1 b2) ; nodec.
   destruct (eqb_spec a1 a2) ; nodec.
   cbn. constructor. subst. reflexivity.
-Defined.
+Qed.
 
 Definition eq_cast_kind (c c' : cast_kind) : bool :=
   match c, c' with
@@ -148,24 +148,38 @@ Definition eq_cast_kind (c c' : cast_kind) : bool :=
 Next Obligation.
   induction x, y. all: cbn. all: nodec.
   all: left. all: reflexivity.
-Defined.
+Qed.
 
-#[global] Instance reflect_case_info : ReflectEq case_info := EqDec_ReflectEq case_info.
+
+
+Definition eqb_case_info
+  (ci ci' : BasicAst.case_info) :=
+  let (ci_ind, ci_npar, ci_relevance) := ci in
+  let (ci_ind', ci_npar', ci_relevance') := ci' in
+  eqb ci_ind ci_ind' && eqb ci_npar ci_npar' && eqb ci_relevance ci_relevance'.
+
+#[global, program] Instance reflect_case_info : ReflectEq case_info :=
+  {| eqb := eqb_case_info |}.
+Next Obligation.
+  intros. destruct x as [ci_ind ci_npar ci_relevance], y as [ci_ind' ci_npar' ci_relevance']. cbn -[eqb].
+  destruct (eqb_spec ci_ind ci_ind'); subst;
+  destruct (eqb_spec ci_npar ci_npar'); subst;
+    destruct (eqb_spec ci_relevance ci_relevance'); subst; constructor; congruence.
+Qed.
 
 Derive NoConfusion NoConfusionHom for sig.
 Derive NoConfusion NoConfusionHom for prod.
 
-Definition eqb_context_decl {term : Type} (eqterm : term -> term -> bool) 
+Definition eqb_context_decl {term : Type} (eqterm : term -> term -> bool)
   (x y : BasicAst.context_decl term) :=
   let (na, b, ty) := x in
   let (na', b', ty') := y in
   eqb na na' && eq_option eqterm b b' && eqterm ty ty'.
 
-#[global] Instance eq_decl_reflect {term} {Ht : ReflectEq term} : ReflectEq (BasicAst.context_decl term).
-Proof.
-  refine {| eqb := eqb_context_decl eqb |}.
-  intros.
-  destruct x as [na b ty], y as [na' b' ty']. cbn -[eqb].
+#[global, program] Instance eq_decl_reflect {term} {Ht : ReflectEq term} : ReflectEq (BasicAst.context_decl term) :=
+  {| eqb := eqb_context_decl eqb |}.
+Next Obligation.
+  intros. destruct x as [na b ty], y as [na' b' ty']. cbn -[eqb].
   change (eq_option eqb b b') with (eqb b b').
   destruct (eqb_spec na na'); subst;
     destruct (eqb_spec b b'); subst;
@@ -219,7 +233,7 @@ Derive NoConfusion EqDec for comparison.
 Lemma string_compare_irrel {s s'} {c} (H H' : string_compare s s' = c) : H = H'.
 Proof.
   apply uip.
-Qed.  
+Qed.
 
 Scheme le_ind_prop := Induction for le Sort Prop.
 
@@ -246,7 +260,7 @@ Proof.
 Qed.
 
 Require Import RelationClasses.
-    
+
 Lemma constraint_lt_irrel (x y : UnivConstraint.t) (l l' : UnivConstraint.lt_ x y) : l = l'.
 Proof.
   revert l'. induction l using constraint_lt_ind_dep.
@@ -266,20 +280,20 @@ Qed.
 
 Module LevelSetsUIP.
   Import LevelSet.Raw.
-  
-  Fixpoint levels_tree_eqb (x y : LevelSet.Raw.t) := 
+
+  Fixpoint levels_tree_eqb (x y : LevelSet.Raw.t) :=
   match x, y with
   | LevelSet.Raw.Leaf, LevelSet.Raw.Leaf => true
-  | LevelSet.Raw.Node h l o r, LevelSet.Raw.Node h' l' o' r' => 
+  | LevelSet.Raw.Node h l o r, LevelSet.Raw.Node h' l' o' r' =>
     eqb h h' && levels_tree_eqb l l' && eqb o o' && levels_tree_eqb r r'
   | _, _ => false
   end.
-  
+
   Scheme levels_tree_rect := Induction for LevelSet.Raw.tree Sort Type.
 
-  #[global] Instance levels_tree_reflect : ReflectEq LevelSet.Raw.t.
-  Proof.
-    refine {| eqb := levels_tree_eqb |}.
+  #[global, program] Instance levels_tree_reflect : ReflectEq LevelSet.Raw.t :=
+   {| eqb := levels_tree_eqb |}.
+  Next Obligation.
     induction x using levels_tree_rect; destruct y; try constructor; auto; try congruence.
     cbn [levels_tree_eqb].
     destruct (eqb_spec t0 t2); try constructor; auto; try congruence.
@@ -287,13 +301,13 @@ Module LevelSetsUIP.
     destruct (eqb_spec t1 t3); try constructor; auto; try congruence.
     destruct (IHx2 y2); try constructor; auto; try congruence.
   Qed.
-  
+
   Derive NoConfusion for LevelSet.Raw.tree.
   Derive Signature for LevelSet.Raw.bst.
-  
+
   Definition eqb_LevelSet x y :=
     eqb (LevelSet.this x) (LevelSet.this y).
-  
+
   Lemma ok_irrel (x : t) (o o' : Ok x) : o = o'.
   Proof.
     unfold Ok in *.
@@ -307,34 +321,34 @@ Module LevelSetsUIP.
       apply lt_level_irrel.
   Qed.
 
-  #[global] Instance reflect_LevelSet : ReflectEq LevelSet.t.
-  Proof.
-    refine {| eqb := eqb_LevelSet |}.
+  #[global,program] Instance reflect_LevelSet : ReflectEq LevelSet.t :=
+   {| eqb := eqb_LevelSet |}.
+  Next Obligation.
     intros [thisx okx] [thisy oky].
     unfold eqb_LevelSet.
     cbn -[eqb].
     destruct (eqb_spec thisx thisy); subst; constructor.
     - f_equal. apply ok_irrel.
     - congruence.
-  Defined.
+  Qed.
 End LevelSetsUIP.
 
 Module ConstraintSetsUIP.
   Import ConstraintSet.Raw.
 
-  Fixpoint cs_tree_eqb (x y : t) := 
+  Fixpoint cs_tree_eqb (x y : t) :=
     match x, y with
     | ConstraintSet.Raw.Leaf, ConstraintSet.Raw.Leaf => true
-    | ConstraintSet.Raw.Node h l o r, ConstraintSet.Raw.Node h' l' o' r' => 
+    | ConstraintSet.Raw.Node h l o r, ConstraintSet.Raw.Node h' l' o' r' =>
       eqb h h' && cs_tree_eqb l l' && eqb o o' && cs_tree_eqb r r'
     | _, _ => false
     end.
 
   Scheme cs_tree_rect := Induction for ConstraintSet.Raw.tree Sort Type.
 
-  #[global] Instance cs_tree_reflect : ReflectEq ConstraintSet.Raw.t.
-  Proof.
-    refine {| eqb := cs_tree_eqb |}.
+  #[global,program] Instance cs_tree_reflect : ReflectEq ConstraintSet.Raw.t :=
+   {| eqb := cs_tree_eqb |}.
+  Next Obligation.
     induction x using cs_tree_rect; destruct y; try constructor; auto; try congruence.
     cbn [cs_tree_eqb].
     destruct (eqb_spec t0 t1); try constructor; auto; try congruence.
@@ -362,16 +376,16 @@ Module ConstraintSetsUIP.
       apply constraint_lt_irrel.
   Qed.
 
-  #[global] Instance reflect_ConstraintSet : ReflectEq ConstraintSet.t.
-  Proof.
-    refine {| eqb := eqb_ConstraintSet |}.
+  #[global,program] Instance reflect_ConstraintSet : ReflectEq ConstraintSet.t :=
+   {| eqb := eqb_ConstraintSet |}.
+  Next Obligation.
     intros [thisx okx] [thisy oky].
     unfold eqb_ConstraintSet. cbn.
     cbn -[eqb].
     destruct (eqb_spec thisx thisy); subst; constructor.
     - f_equal. apply ok_irrel.
     - congruence.
-  Defined.
+  Qed.
 
 End ConstraintSetsUIP.
 
@@ -388,13 +402,13 @@ Definition eqb_universes_decl x y :=
   | Polymorphic_ctx cx, Polymorphic_ctx cy => eqb cx cy
   | _, _ => false
   end.
-  
-#[global] Instance reflect_universes_decl : ReflectEq universes_decl.
-Proof.
-  refine {| eqb := eqb_universes_decl |}.
-  unfold eqb_universes_decl.
-  intros [] []; finish_reflect.
-Defined.
+
+#[global,program] Instance reflect_universes_decl : ReflectEq universes_decl :=
+ {| eqb := eqb_universes_decl |}.
+ Next Obligation.
+   unfold eqb_universes_decl.
+   intros [] []; finish_reflect.
+Qed.
 
 Definition eqb_allowed_eliminations x y :=
   match x, y with
@@ -405,11 +419,11 @@ Definition eqb_allowed_eliminations x y :=
   | _, _ => false
   end.
 
-#[global] Instance reflect_allowed_eliminations : ReflectEq allowed_eliminations.
-Proof.
-  refine {| eqb := eqb_allowed_eliminations |}.
-  intros [] []; simpl; constructor; congruence.
-Defined.
+#[global,program] Instance reflect_allowed_eliminations : ReflectEq allowed_eliminations :=
+ {| eqb := eqb_allowed_eliminations |}.
+Next Obligation.
+ intros [] []; simpl; constructor; congruence.
+Qed.
 
 Local Infix "==?" := eqb (at level 20).
 
@@ -421,8 +435,8 @@ Definition eqb_Variance x y :=
   | _, _ => false
   end.
 
-#[global] Instance reflect_Variance : ReflectEq Variance.t.
-Proof.
-  refine {| eqb := eqb_Variance |}.
+#[global,program] Instance reflect_Variance : ReflectEq Variance.t :=
+ {| eqb := eqb_Variance |}.
+Next Obligation.
   intros [] []; constructor; congruence.
-Defined.
+Qed.
