test-suite/erasure_live_test.v
@@ -1,12 +1,14 @@
 From Coq Require Import Recdef.
 From MetaCoq.Template Require Import TemplateMonad Loader.
 (* From MetaCoq.SafeChecker Require Import SafeTemplateChecker. *)
-From MetaCoq.PCUIC Require Import PCUICAstUtils.
+From MetaCoq.PCUIC Require Import PCUICEquality PCUICAst PCUICReflect PCUICSafeLemmata PCUICTyping PCUICNormal PCUICAstUtils PCUICSN TemplateToPCUIC PCUICToTemplate.
+
 From MetaCoq.Erasure Require Import Erasure.
+
 From Coq Require Import String.
 Local Open Scope string_scope.
 
-From MetaCoq.Template Require Import utils.
+From MetaCoq.Template Require Import utils config.
 Import MCMonadNotation.
 Unset MetaCoq Debug.
 (* We're doing erasure assuming no Prop <= Type rule and lets can appear in constructor types. *)
